make the calculation of "handled" functions implicit with respect to a given extension (in particular, "handled" need no longer be a finite list of external functions).
this makes it possible to construct extensions that handle 
countably many external functions.  it also simplifies some 
definitions and obviates some stupid axioms in the defn. of 
extension.

veric/extension.v
@@ -13,137 +13,113 @@ Require Import Integers.
 
 Set Implicit Arguments.
 
-Module TruePropCoercion.
-Definition is_true (b: bool) := b=true.
-Coercion is_true: bool >-> Sortclass.
-End TruePropCoercion.
-Import TruePropCoercion.
-
 (** * Extensions *)
 
-Module Extension. Section Extension.
- Variables
-  (G: Type) (** global environments of extended semantics *)
-  (D: Type) (** extension initialization data *)
-  (xT: Type) (** corestates of extended semantics *)
-  (gT: nat -> Type) (** global environments of core semantics *)
-  (cT: nat -> Type) (** corestates of core semantics *)
-  (M: Type) (** memories *)
-  (dT: nat -> Type) (** initialization data *)
-  (Z: Type) (** external states *)
-  (Zint: Type) (** portion of Z implemented by extension *)
-  (Zext: Type) (** portion of Z external to extension *)
-
-  (esem: CoreSemantics G xT M D) (** extended semantics *)
-  (csem: forall i:nat, CoreSemantics (gT i) (cT i) M (dT i)) (** a set of core semantics *)
-
-  (csig: ef_ext_spec M Z) (** client signature *)
-  (esig: ef_ext_spec M Zext) (** extension signature *)
-
-  (handled: list AST.external_function). (** functions handled by this extension *)
-
- Local Open Scope nat_scope.
-
- Notation IN := (ListSet.set_mem extfunct_eqdec).
- Notation NOTIN := (fun ef l => ListSet.set_mem extfunct_eqdec ef l = false).
- Notation DIFF := (ListSet.set_diff extfunct_eqdec).
+Module Extension. Section Extension. Variables
+ (M: Type) (** memories *)
+ (Z: Type) (** external states *)
+ (Zint: Type) (** portion of Z implemented by extension *)
+ (Zext: Type) (** portion of Z external to extension *)
+ (G: Type) (** global environments of extended semantics *)
+ (D: Type) (** extension initialization data *)
+ (xT: Type) (** corestates of extended semantics *)
+ (esem: CoreSemantics G xT M D) (** extended semantics *)
+ (esig: ef_ext_spec M Zext) (** extension signature *)
+ (gT: nat -> Type) (** global environments of core semantics *)
+ (dT: nat -> Type) (** initialization data *)
+ (cT: nat -> Type) (** corestates of core semantics *)
+ (csem: forall i:nat, CoreSemantics (gT i) (cT i) M (dT i)) (** a set of core semantics *)
+ (csig: ef_ext_spec M Z). (** client signature *)
 
  Record Sig := Make {
- (** Generalized projection of genv, core [i] from state [s] *)
   proj_max_cores: xT -> nat;
   proj_core: forall i:nat, xT -> option (cT i); 
-  proj_core_proj_max: forall i s, i >= proj_max_cores s -> proj_core i s = None;
-  active : xT -> nat; (** The active (i.e., currently scheduled) core *)
-  active_proj_core : forall s, exists c, proj_core (active s) s = Some c;
-  proj_zint: xT -> Zint; (** Type [xT] embeds [Zint]. *)
+  proj_core_max: forall i s, i>=proj_max_cores s -> proj_core i s=None;
+  active : xT -> nat; 
+  active_proj_core : forall s, exists c, proj_core (active s) s=Some c;
+  proj_zint: xT -> Zint; 
   proj_zext: Z -> Zext;
   zmult: Zint -> Zext -> Z;
   zmult_proj: forall zint zext, proj_zext (zmult zint zext)=zext;
-
- (** When a core is AtExternal but the extension is not, the function on which 
-    the core is blocked is handled by the extension. *)
-  notat_external_handled: forall s c ef args sig,
-   proj_core (active s) s = Some c -> 
-   at_external (csem (active s)) c = Some (ef, sig, args) -> 
-   at_external esem s = None -> IN ef handled;
-
- (** Functions on which the extension is blocked are not handled. *)
-  at_external_not_handled: forall s ef args sig,
-   at_external esem s = Some (ef, sig, args) -> NOTIN ef handled;
-
- (** Implemented "external" state is unchanged after truly external calls. *)
-  ext_upd_at_external : forall ef sig args ret s s',
+ 
+  zint_invar_after_external: forall ef sig args ret s s',
    at_external esem s = Some (ef, sig, args) -> 
    after_external esem ret s = Some s' -> proj_zint s=proj_zint s';
-   
- (** [esem] and [csem] are signature linkable *)
-  esem_csem_linkable: linkable proj_zext handled csig esig
+
+  handled (ef: AST.external_function) :=
+   forall (s: xT) (c: cT (active s)) sig args,
+    proj_core (active s) s = Some c ->
+    at_external (csem (active s)) c = Some (ef, sig, args) ->
+    at_external esem s = None;
+
+  linkable: linkable proj_zext handled csig esig;
+
+  handled_invar: 
+   forall s c s' c' ef sig args sig' args',
+    proj_core (active s) s = Some c ->
+    at_external (csem (active s)) c = Some (ef, sig, args) ->
+    at_external esem s = None -> 
+    proj_core (active s') s' = Some c' ->
+    at_external (csem (active s')) c' = Some (ef, sig', args') ->
+    at_external esem s' = None
  }.
 
 End Extension. End Extension.
+
+Implicit Arguments Extension.Sig [M G D xT].
 Implicit Arguments Extension.Make [G xT cT M D Z Zint Zext].
 
 (** * Safe Extensions *)
 
-Section SafeExtension.
- Variables
-  (G: Type) (** global environments *)
-  (D: Type) (** initialization data *)
-  (xT: Type) (** corestates of extended semantics *)
-  (gT: nat -> Type) (** global environments of the core semantics *)
-  (cT: nat -> Type) (** corestates of core semantics *)
-  (M: Type) (** memories *)
-  (dT: nat -> Type) (** initialization data *)
-  (Z: Type) (** external states *)
-  (Zint: Type) (** portion of Z implemented by extension *)
-  (Zext: Type) (** portion of Z external to extension *)
-
-  (esem: CoreSemantics G xT M D) (** extended semantics *)
-  (csem: forall i:nat, CoreSemantics (gT i) (cT i) M (dT i)) (** a set of core semantics *)
-
-  (csig: ef_ext_spec M Z) (** client signature *)
-  (esig: ef_ext_spec M Zext) (** extension signature *)
-  (handled: list AST.external_function). (** functions handled by this extension *)
+Section SafeExtension. Variables
+ (M: Type) (** memories *)
+ (Z: Type) (** external states *)
+ (Zint: Type) (** portion of Z implemented by extension *)
+ (Zext: Type) (** portion of Z external to extension *)
+ (G: Type) (** global environments of extended semantics *)
+ (D: Type) (** extension initialization data *)
+ (xT: Type) (** corestates of extended semantics *)
+ (esem: CoreSemantics G xT M D) (** extended semantics *)
+ (esig: ef_ext_spec M Zext) (** extension signature *)
+ (gT: nat -> Type) (** global environments of core semantics *)
+ (dT: nat -> Type) (** initialization data *)
+ (cT: nat -> Type) (** corestates of core semantics *)
+ (csem: forall i:nat, CoreSemantics (gT i) (cT i) M (dT i)) (** a set of core semantics *)
+ (csig: ef_ext_spec M Z). (** client signature *)
 
  Variables (ge: G) (genv_map : forall i:nat, gT i).
 
  Import Extension.
 
- Definition all_safe (E: Sig gT cT dT Zint esem csem csig esig handled)
-  (n: nat) (z: Z) (w: xT) (m: M) :=
-     forall i c, proj_core E i w = Some c -> 
-       safeN (csem i) csig (genv_map i) n z c m.
+ Definition all_safe (E: Sig Z Zint Zext esem esig gT dT cT csem csig)
+   (n: nat) (z: Z) (w: xT) (m: M) :=
+  forall i c, proj_core E i w = Some c -> 
+  safeN (csem i) csig (genv_map i) n z c m.
 
- (** All-safety implies safeN. *)
- Definition safe_extension (E: Sig gT cT dT Zint esem csem csig esig handled) :=
-  forall n s m z, 
-    all_safe E n (zmult E (proj_zint E s) z) s m -> 
-    safeN esem (link_ext_spec handled esig) ge n z s m.
+ Definition safe_extension (E: Sig Z Zint Zext esem esig gT dT cT csem csig) :=
+  forall n s m z, all_safe E n (zmult E (proj_zint E s) z) s m -> 
+  safeN esem (link_ext_spec (handled E) esig) ge n z s m.
 
 End SafeExtension.
 
-Module SafetyInvariant. Section SafetyInvariant.
- Variables
-  (G: Type) (** global environments *)
-  (D: Type) (** initialization data *)
-  (xT: Type) (** corestates of extended semantics *)
-  (gT: nat -> Type) (** global environments of the core semantics *)
-  (cT: nat -> Type) (** corestates of core semantics *)
-  (M: Type) (** memories *)
-  (dT: nat -> Type) (** initialization data *)
-  (Z: Type) (** external states *)
-  (Zint: Type) (** portion of Z implemented by extension *)
-  (Zext: Type) (** portion of Z external to extension *)
-
-  (esem: CoreSemantics G xT M D) (** extended semantics *)
-  (csem: forall i:nat, CoreSemantics (gT i) (cT i) M (dT i)) (** a set of core semantics *)
-
-  (csig: ef_ext_spec M Z) (** client signature *)
-  (esig: ef_ext_spec M Zext) (** extension signature *)
-  (handled: list AST.external_function). (** functions handled by this extension *)
+Module SafetyInvariant. Section SafetyInvariant. Variables
+ (M: Type) (** memories *)
+ (Z: Type) (** external states *)
+ (Zint: Type) (** portion of Z implemented by extension *)
+ (Zext: Type) (** portion of Z external to extension *)
+ (G: Type) (** global environments of extended semantics *)
+ (D: Type) (** extension initialization data *)
+ (xT: Type) (** corestates of extended semantics *)
+ (esem: CoreSemantics G xT M D) (** extended semantics *)
+ (esig: ef_ext_spec M Zext) (** extension signature *)
+ (gT: nat -> Type) (** global environments of core semantics *)
+ (dT: nat -> Type) (** initialization data *)
+ (cT: nat -> Type) (** corestates of core semantics *)
+ (csem: forall i:nat, CoreSemantics (gT i) (cT i) M (dT i)) (** a set of core semantics *)
+ (csig: ef_ext_spec M Z). (** client signature *)
 
  Variables (ge: G) (genv_map : forall i:nat, gT i).
- Variable E: Extension.Sig gT cT dT Zint esem csem csig esig handled.
+ Variable E: Extension.Sig Z Zint Zext esem esig gT dT cT csem csig.
 
 Definition proj_zint := E.(Extension.proj_zint). 
 Coercion proj_zint : xT >-> Zint.
@@ -157,9 +133,7 @@ Notation "zint \o zext" := (E.(Extension.zmult) zint zext)
   (at level 66, left associativity). 
 Notation ACTIVE := (E.(Extension.active)).
 Notation active_proj_core := E.(Extension.active_proj_core).
-Notation notat_external_handled := E.(Extension.notat_external_handled).
-Notation at_external_not_handled := E.(Extension.at_external_not_handled).
-Notation ext_upd_at_external := E.(Extension.ext_upd_at_external).
+Notation zint_invar_after_external := E.(Extension.zint_invar_after_external).
 
 Inductive safety_invariant: Type := SafetyInvariant: forall 
  (** Coresteps preserve the all-safety invariant. *)
@@ -185,14 +159,13 @@ Inductive safety_invariant: Type := SafetyInvariant: forall
      (c': cT (ACTIVE s)) ef sig args P Q x, 
   let i := ACTIVE s in PROJ_CORE i s = Some c -> 
    at_external (csem i) c = Some (ef, sig, args) -> 
-   ListSet.set_mem extfunct_eqdec ef handled = true -> 
+   Extension.handled E ef -> 
    spec_of ef csig = (P, Q) -> 
    P x (sig_args sig) args (s \o z) m -> 
    corestep esem ge s m s' m' -> 
    PROJ_CORE i s' = Some c' -> 
     ((at_external (csem i) c' = Some (ef, sig, args) /\ 
-      P x (sig_args sig) args (s' \o z) m' /\
-      (forall j, ACTIVE s' = j -> i <> j)) \/
+      P x (sig_args sig) args (s' \o z) m' /\ i <> ACTIVE s') \/
     (exists ret, after_external (csem i) ret c = Some c' /\ 
       Q x (sig_res sig) ret (s' \o z) m')))
 
@@ -275,32 +248,29 @@ Inductive safety_invariant: Type := SafetyInvariant: forall
 
 End SafetyInvariant. End SafetyInvariant.
 
-Module EXTENSION_SAFETY. Section EXTENSION_SAFETY.
- Variables
-  (G: Type) (** global environments *)
-  (D: Type) (** initialization data *)
-  (xT: Type) (** corestates of extended semantics *)
-  (gT: nat -> Type) (** global environments of the core semantics *)
-  (cT: nat -> Type) (** corestates of core semantics *)
-  (M: Type) (** memories *)
-  (dT: nat -> Type) (** initialization data *)
-  (Z: Type) (** external states *)
-  (Zint: Type) (** portion of Z implemented by extension *)
-  (Zext: Type) (** portion of Z external to extension *)
-
-  (esem: CoreSemantics G xT M D) (** extended semantics *)
-  (csem: forall i:nat, CoreSemantics (gT i) (cT i) M (dT i)) (** a set of core semantics *)
-
-  (csig: ef_ext_spec M Z) (** client signature *)
-  (esig: ef_ext_spec M Zext) (** extension signature *)
-  (handled: list AST.external_function). (** functions handled by this extension *)
+Module EXTENSION_SAFETY. Section EXTENSION_SAFETY. Variables
+ (M: Type) (** memories *)
+ (Z: Type) (** external states *)
+ (Zint: Type) (** portion of Z implemented by extension *)
+ (Zext: Type) (** portion of Z external to extension *)
+ (G: Type) (** global environments of extended semantics *)
+ (D: Type) (** extension initialization data *)
+ (xT: Type) (** corestates of extended semantics *)
+ (esem: CoreSemantics G xT M D) (** extended semantics *)
+ (esig: ef_ext_spec M Zext) (** extension signature *)
+ (gT: nat -> Type) (** global environments of core semantics *)
+ (dT: nat -> Type) (** initialization data *)
+ (cT: nat -> Type) (** corestates of core semantics *)
+ (csem: forall i:nat, CoreSemantics (gT i) (cT i) M (dT i)) (** a set of core semantics *)
+ (csig: ef_ext_spec M Z). (** client signature *)
 
  Variables (ge: G) (genv_map : forall i:nat, gT i).
- Variable E: Extension.Sig gT cT dT Zint esem csem csig esig handled.
+ Variable E: Extension.Sig Z Zint Zext esem esig gT dT cT csem csig.
 
 Import SafetyInvariant.
 
-Record Sig := Make {_: safety_invariant ge genv_map E -> safe_extension ge genv_map E}.
+Record Sig := Make {_: safety_invariant ge genv_map E -> 
+                       safe_extension ge genv_map E}.
 
 End EXTENSION_SAFETY. End EXTENSION_SAFETY.
 
@@ -308,28 +278,24 @@ End EXTENSION_SAFETY. End EXTENSION_SAFETY.
    inner cores. Perhaps some of these conditions could be merged with those for
    "safe" extensions. *)
 
-Section CoreCompatible.
- Variables
-  (G: Type) (** global environments *)
-  (D: Type) (** initialization data *)
-  (xT: Type) (** corestates of extended semantics *)
-  (gT: nat -> Type) (** global environments of the core semantics *)
-  (cT: nat -> Type) (** corestates of core semantics *)
-  (M: Type) (** memories *)
-  (dT: nat -> Type) (** initialization data *)
-  (Z: Type) (** external states *)
-  (Zint: Type) (** portion of Z implemented by extension *)
-  (Zext: Type) (** portion of Z external to extension *)
+Section CoreCompatible. Variables 
+ (M: Type) (** memories *)
+ (Z: Type) (** external states *)
+ (Zint: Type) (** portion of Z implemented by extension *)
+ (Zext: Type) (** portion of Z external to extension *)
+ (G: Type) (** global environments of extended semantics *)
+ (D: Type) (** extension initialization data *)
+ (xT: Type) (** corestates of extended semantics *)
+ (esem: CoreSemantics G xT M D) (** extended semantics *)
+ (esig: ef_ext_spec M Zext) (** extension signature *)
+ (gT: nat -> Type) (** global environments of core semantics *)
+ (dT: nat -> Type) (** initialization data *)
+ (cT: nat -> Type) (** corestates of core semantics *)
+ (csem: forall i:nat, CoreSemantics (gT i) (cT i) M (dT i)) (** a set of core semantics *)
+ (csig: ef_ext_spec M Z). (** client signature *)
 
-  (esem: CoreSemantics G xT M D) (** extended semantics *)
-  (csem: forall i:nat, CoreSemantics (gT i) (cT i) M (dT i)) (** a set of core semantics *)
-
-  (csig: ef_ext_spec M Z) (** client signature *)
-  (esig: ef_ext_spec M Zext) (** extension signature *)
-  (handled: list AST.external_function). (** functions handled by this extension *)
-
-Variables (ge: G) (genv_map : forall i:nat, gT i).
-Variable E: Extension.Sig gT cT dT Zint esem csem csig esig handled.
+ Variables (ge: G) (genv_map : forall i:nat, gT i).
+ Variable E: Extension.Sig Z Zint Zext esem esig gT dT cT csem csig.
 
 Import Extension.
 
