veric/extspec.v
@@ -25,6 +25,11 @@ Proof. intros ef1 ef2; repeat decide equality; apply Address.EqDec_int. Qed.
 
 Set Implicit Arguments.
 
+Definition ef_ext_spec (M Z: Type) := external_specification M AST.external_function Z.
+
+Definition spec_of (M Z: Type) (ef: AST.external_function) (Sigma: ef_ext_spec M Z) :=
+  (ext_spec_pre Sigma ef, ext_spec_post Sigma ef).
+
 Section LinkExtSpec.
 Notation IN := (ListSet.set_mem extfunct_eqdec).
 Notation NOTIN := (fun ef l => ListSet.set_mem extfunct_eqdec ef l = false).
@@ -42,32 +47,26 @@ Qed.
 (** Linking external specification [Sigma] with an extension implementing
    functions in [handled] *)
 
-Definition link_ext_spec (M Z: Type) (handled: list AST.external_function) 
+Definition link_ext_spec (M Z: Type) (handled: AST.external_function -> Prop) 
   (Sigma: external_specification M AST.external_function Z) :=
   Build_external_specification M AST.external_function Z
     (ext_spec_type Sigma)
     (fun (ef: AST.external_function) (x: ext_spec_type Sigma ef)
          (tys: list typ) (args: list val) (z: Z) (m: M) => 
-             if ListSet.set_mem extfunct_eqdec ef handled then False 
-             else ext_spec_pre Sigma ef x tys args z m)
+             ~handled ef /\ ext_spec_pre Sigma ef x tys args z m)
     (fun (ef: AST.external_function) (x: ext_spec_type Sigma ef)
          (ty: option typ) (ret: option val) (z: Z) (m: M) => 
-             if ListSet.set_mem extfunct_eqdec ef handled then True
-             else ext_spec_post Sigma ef x ty ret z m).
+             handled ef \/ ext_spec_post Sigma ef x ty ret z m).
 
 (** A client signature is linkable with an extension signature when each
    extension function specification ef:{P}{Q} is a subtype of the
    specification ef:{P'}{Q'} assumed by client. *)
 
-Definition ef_ext_spec (M Z: Type) := external_specification M AST.external_function Z.
-
-Definition spec_of (M Z: Type) (ef: AST.external_function) (Sigma: ef_ext_spec M Z) :=
-  (ext_spec_pre Sigma ef, ext_spec_post Sigma ef).
-
 Definition linkable (M Z Zext: Type) (proj_zext: Z -> Zext)
-      (handled: list AST.external_function) 
+      (handled: AST.external_function -> Prop) 
       (csig: ef_ext_spec M Z) (ext_sig: ef_ext_spec M Zext) := 
   forall ef P Q P' Q', 
+    ~handled ef -> 
     spec_of ef ext_sig = (P, Q) -> 
     spec_of ef csig = (P', Q') -> 
     forall x' tys args m z, P' x' tys args z m -> 
@@ -75,3 +74,4 @@ Definition linkable (M Z Zext: Type) (proj_zext: Z -> Zext)
       forall ty ret m' z', Q x ty ret (proj_zext z') m' -> Q' x' ty ret z' m'.
 
 End LinkExtSpec.
+
